complete encoding function

Varint.fst
@@ -8,6 +8,7 @@ open FStar.UInt64
 open FStar.Int.Cast.Full
 open FStar.Seq
 open FStar.List.Tot
+open FStar.Mul
 
 module U = FStar.UInt
 module U8 = FStar.UInt8
@@ -25,41 +26,33 @@ let rec valid (v:list UInt8.t) : bool =
        which is equivalent to the number fitting into 7 bits *)
   | msb :: [] -> UInt.fits (U8.v msb) 7
     (* Otherwise the continuation bit should be one *)
-  | msb :: rest -> (U8.(msb &^ 0x80uy) = 128uy) && valid rest
+    (* Note that U.msb is "most significant bit" while the msb is the patter match is "most significant byte" *)
+  | msb :: rest -> U.msb (U8.v msb) && valid rest
 
 let varint = v:list UInt8.t{length v >= 1 /\ valid v}
 
-
-// let rec encode (l:pos{l % 8 = 0}) (x: U.uint_t l) : Tot varint (decreases l) = 
-//   assert l > 7; 
-//   let nextByte = U.logand x (U.to_uint_t l 0x7F) in 
-//   let rest = U.(shift_right x 7) in
-//   UInt.logand_le x (U.to_uint_t l 0x7F);
-//   assert nextByte < 128;
-//   assert U.fits nextByte 8;
-//   if rest = U.zero l then
-//     [U8.uint_to_t nextByte]
-//   else 
-//     let nextByte = U8.(uint_to_t nextByte |^ 128uy) in 
-//     [nextByte]
 
 let rec encode (x: U64.t) : Tot varint (decreases (U64.v x)) = 
   let nextByte = Cast.uint64_to_uint8 (U64.logand x 0x7FuL) in 
   let rest = U64.(x >>^ 7ul) in
   UInt.logand_le (U64.v x) 0x7F;
   assert UInt.fits U8.(v nextByte) 7;
-  if rest = 0uL then 
+  if U64.(lte rest 0uL) then 
     [nextByte]
   else 
-    let nextByte = U8.(nextByte |^ 128uy) in
-    assume U64.v rest < U64.v x;
+    let nextByte = U8.(nextByte +^ 128uy) in
+    UInt.shift_right_value_lemma (U64.v x) 7;
+    assert op_Division (U64.v x) 128 = (U64.v rest);
     let restEnc = encode rest in
-    assert valid restEnc;
-    assume U8.(nextByte &^ 0x80uy) = 128uy;
+    assert (U8.v nextByte) >= 128;
+    UInt.lemma_msb_pow2 (U8.v nextByte);
     List.append [nextByte] restEnc
-  
 
-let rec decode (bs:varint) (x:erased UInt64.t) : y:UInt64.t{(requires bs == encode(x)) (ensures y == x)}
-  = 0
+let rec decode (bs:varint) (x:erased U64.t{bs == encode(x)}) : y:U64.t{y == reveal x} =
+  let nextByte = hd bs in
+  match U.msb (U8.v nextByte) with 
+  | true -> Cast.uint8_to_uint64 nextByte
+  | false -> 0uL
+  
 
 (* Relevant F* code in ASN1*: ANS1.Spec.IdentifierU32.fst *)
